Search correctness

src/DenotationalSem.v
@@ -4,35 +4,83 @@ Require Import Stream.
 Require Import Unify.
 Require Import MiniKanrenSyntax.
 Require Import OperationalSem.
+Require Import Omega.
 
 Definition gt_fun : Set := name -> ground_term.
 
-Fixpoint apply_gt_fun (f : gt_fun) (t : term) : term :=
-  match t with
-  | Var x => proj1_sig (f x)
-  | Cst n => Cst n
-  | Con n l r => Con n (apply_gt_fun f l) (apply_gt_fun f r)
-  end.
+Definition gt_eq (gt1 : ground_term) (gt2 : ground_term) : Prop :=
+  proj1_sig gt1 = proj1_sig gt2.
 
-Variable P : spec.
+Definition gt_fun_eq (f1 : gt_fun) (f2 : gt_fun) : Prop :=
+  forall x, gt_eq (f1 x) (f2 x).
+
+Fixpoint apply_gt_fun (f : gt_fun) (t : term) : ground_term.
+refine (
+  match t with
+  | Var x => f x
+  | Cst n => exist _ (Cst n) eq_refl
+  | Con n l r => match apply_gt_fun f l, apply_gt_fun f r with
+                 | exist _ lt lg, exist _ rt rg => exist _ (Con n lt rt) _
+                 end
+  end
+).
+simpl. rewrite lg. rewrite rg. reflexivity.
+Defined.
+
+Lemma gt_fun_eq_apply (f1 f2 : gt_fun) (t : term) (feq : gt_fun_eq f1 f2) :
+  gt_eq (apply_gt_fun f1 t) (apply_gt_fun f2 t).
+Proof.
+  induction t.
+  { simpl. auto. }
+  { reflexivity. }
+  { red. simpl.
+    destruct (apply_gt_fun f1 t1). destruct (apply_gt_fun f1 t2).
+    destruct (apply_gt_fun f2 t1). destruct (apply_gt_fun f2 t2).
+    simpl.
+    red in IHt1. simpl in IHt1.
+    red in IHt2. simpl in IHt2.
+    subst. auto. }
+Qed.
+
+Definition subst_gt_fun_compose (s : subst) (f : gt_fun) : gt_fun :=
+  fun x => apply_gt_fun f (apply_subst s (Var x)).
+
+Lemma gt_fun_apply_compose (s : subst) (f : gt_fun) (t : term) :
+  gt_eq (apply_gt_fun (subst_gt_fun_compose s f) t) (apply_gt_fun f (apply_subst s t)).
+Proof.
+  induction t.
+  { reflexivity. }
+  { reflexivity. }
+  { red. simpl.
+    destruct (apply_gt_fun (subst_gt_fun_compose s f) t1).
+    destruct (apply_gt_fun (subst_gt_fun_compose s f) t2).
+    destruct (apply_gt_fun f (apply_subst s t1)).
+    destruct (apply_gt_fun f (apply_subst s t2)).
+    simpl.
+    red in IHt1. simpl in IHt1.
+    red in IHt2. simpl in IHt2.
+    subst. auto. }
+Qed.
 
 (* Simple variant *)
 Inductive in_denotational_sem_goal : goal -> gt_fun -> Prop :=
-| dsgUnify  : forall f t1 t2 (UnH : apply_gt_fun f t1 = apply_gt_fun f t2),
-                            in_denotational_sem_goal (Unify t1 t2) f
+| dsgUnify  : forall f t1 t2 (UnH : gt_eq (apply_gt_fun f t1) (apply_gt_fun f t2)),
+                             in_denotational_sem_goal (Unify t1 t2) f
 | dsgDisjL  : forall f g1 g2 (Hg : in_denotational_sem_goal g1 f),
-                            in_denotational_sem_goal (Disj g1 g2) f
+                             in_denotational_sem_goal (Disj g1 g2) f
 | dsgDisjR  : forall f g1 g2 (Hg : in_denotational_sem_goal g2 f),
-                            in_denotational_sem_goal (Disj g1 g2) f
+                             in_denotational_sem_goal (Disj g1 g2) f
 | dsgConj   : forall f g1 g2 (Hg1 : in_denotational_sem_goal g1 f)
-                            (Hg2 : in_denotational_sem_goal g2 f),
-                            in_denotational_sem_goal (Conj g1 g2) f
-| dsgFresh  : forall f fn a fg (fvH : forall n, ~ In a (fv_goal n (Fresh fg)))
-                              (Hg : in_denotational_sem_goal (fg a) fn)
-                              (Hease : forall (x : name) (neq : x <> a), fn x = f x),
-                              in_denotational_sem_goal (Fresh fg) f
-| dsgInvoke : forall r t f (Hbody : in_denotational_sem_goal (proj1_sig (P r) t) f),
-                          in_denotational_sem_goal (Invoke r t) f.
+                             (Hg2 : in_denotational_sem_goal g2 f),
+                             in_denotational_sem_goal (Conj g1 g2) f
+| dsgFresh  : forall f fn a fg (fvH : ~ is_fv_of_goal a (Fresh fg))
+                               (Hg : in_denotational_sem_goal (fg a) fn)
+                               (Hease : forall (x : name) (neq : x <> a), fn x = f x),
+                               in_denotational_sem_goal (Fresh fg) f
+| dsgInvoke : forall r t f (Hbody : in_denotational_sem_goal (proj1_sig (OperationalSem.P r) t) f),
+                           in_denotational_sem_goal (Invoke r t) f.
+
+Hint Constructors in_denotational_sem_goal.
 
 (**)
 
@@ -65,7 +113,7 @@ Definition in_denotational_sem (f : gt_fun) (g : goal) : Prop := exists lev, in_
 ( **)
 
 Definition in_denotational_sem_subst (s : subst) (f : gt_fun) : Prop :=
-  exists (f' : gt_fun), forall (x : name), apply_gt_fun f' (apply_subst s (Var x)) = proj1_sig (f x).
+  exists (f' : gt_fun), gt_fun_eq (subst_gt_fun_compose s f') f.
 
 Inductive in_denotational_sem_state' : state' -> gt_fun -> Prop :=
 | dsst'Leaf : forall g s n f (Hgoal : in_denotational_sem_goal g f)
@@ -73,18 +121,107 @@ Inductive in_denotational_sem_state' : state' -> gt_fun -> Prop :=
                              in_denotational_sem_state' (Leaf g s n) f
 | dsst'SumL : forall st1' st2' f (Hst1' : in_denotational_sem_state' st1' f),
                                  in_denotational_sem_state' (Sum st1' st2') f
-| dsst'SumR : forall st1' st2' f (Hst1' : in_denotational_sem_state' st2' f),
+| dsst'SumR : forall st1' st2' f (Hst2' : in_denotational_sem_state' st2' f),
                                  in_denotational_sem_state' (Sum st1' st2') f
 | dsst'Prod : forall st' g f (Hgoal : in_denotational_sem_goal g f)
                              (Hst' : in_denotational_sem_state' st' f),
                              in_denotational_sem_state' (Prod st' g) f.
 
+Hint Constructors in_denotational_sem_state'.
+
 Inductive in_denotational_sem_state : state -> gt_fun -> Prop :=
 | dsstState : forall st' f (Hst' : in_denotational_sem_state' st' f),
                            in_denotational_sem_state (State st') f.
 
+Hint Constructors in_denotational_sem_state.
+
 Definition in_denotational_analog (t : trace) (f : gt_fun) : Prop :=
   exists (s : subst) (n : nat), in_stream (Answer s n) t /\ in_denotational_sem_subst s f.
+
+Lemma answer_correct
+      (s : subst)
+      (n : nat)
+      (f : gt_fun)
+      (HInDS : in_denotational_sem_subst s f)
+      (st' : state')
+      (st : state)
+      (EV : eval_step st' (Answer s n) st) :
+      in_denotational_sem_state' st' f.
+Proof.
+  remember (Answer s n) as l.
+  induction EV; good_inversion Heql.
+  2, 3: auto.
+  destruct HInDS as [f' ff'_con].
+  constructor.
+  { constructor. red.
+    specialize (gt_fun_eq_apply _ _ t1 ff'_con). intro. rewrite <- H.
+    specialize (gt_fun_eq_apply _ _ t2 ff'_con). intro. rewrite <- H0.
+    rewrite gt_fun_apply_compose. rewrite gt_fun_apply_compose.
+    rewrite compose_correctness. rewrite compose_correctness.
+    apply unify_unifies in u. rewrite u. reflexivity. }
+  { red. exists (subst_gt_fun_compose s' f').
+    red. intros. red.
+    red in ff'_con. specialize (ff'_con x). red in ff'_con.
+    rewrite <- ff'_con. unfold subst_gt_fun_compose.
+    replace (fun x0 : name => apply_gt_fun f' (apply_subst s' (Var x0)))
+      with (subst_gt_fun_compose s' f').
+    2: reflexivity.
+    rewrite gt_fun_apply_compose. rewrite compose_correctness.
+    reflexivity. }
+Qed.
+
+Lemma next_state_correct
+      (f : gt_fun)
+      (st : state)
+      (HInDS : in_denotational_sem_state st f)
+      (st' : state')
+      (wfState : well_formed_state' st')
+      (h : label)
+      (EV : eval_step st' h st) :
+      in_denotational_sem_state' st' f.
+Proof.
+  induction EV; good_inversion HInDS.
+  { good_inversion Hst'.
+    { good_inversion Hst1'; constructor; auto. }
+    { good_inversion Hst2'; constructor; auto. } }
+  { good_inversion Hst'. good_inversion Hst'0. auto. }
+  { good_inversion wfState. good_inversion Hst'.
+    constructor; auto. econstructor; eauto.
+    intros HIn. apply freshCorrect in HIn. omega. }
+  { good_inversion Hst'. auto. }
+  { auto. }
+  { good_inversion wfState. good_inversion Hst'; auto. }
+  { good_inversion Hst'. constructor; auto.
+    eapply answer_correct; eauto. }
+  { good_inversion wfState. good_inversion Hst'. auto. }
+  { good_inversion wfState. good_inversion Hst'.
+    { good_inversion Hst1'. constructor; auto.
+      eapply answer_correct; eauto. }
+    { good_inversion Hst2'. auto. } }
+Qed.
+
+Lemma search_correctness_generalized
+      (st   : state)
+      (wfSt : well_formed_state st)
+      (f    : gt_fun)
+      (t    : trace)
+      (HOP  : op_sem st t)
+      (HDA  : in_denotational_analog t f) :
+      in_denotational_sem_state st f.
+Proof.
+  revert HOP wfSt. revert st.
+  red in HDA. destruct HDA as [s [n [HInStr HInDS]]].
+  remember (Answer s n) as l. induction HInStr.
+  { intros. inversion HOP; clear HOP; subst.
+    constructor. eapply answer_correct; eauto. }
+  { specialize (IHHInStr Heql). intros.
+    inversion HOP; clear HOP; subst.
+    inversion wfSt; clear wfSt; subst.
+    specialize (well_formedness_preservation _ _ _ EV wfState).
+    intro wf_st0.
+    specialize (IHHInStr st0 OP wf_st0).
+    constructor. eapply next_state_correct; eauto. }
+Qed.
 
 Fixpoint first_nats (k : nat) : list nat :=
   match k with
@@ -92,12 +229,26 @@ Fixpoint first_nats (k : nat) : list nat :=
   | S n => n :: first_nats n
   end.
 
-Lemma correctness
+Lemma first_nats_less (n k : nat) (H : In n (first_nats k)) : n < k.
+Proof.
+  induction k.
+  { inversion H. }
+  { inversion H. { omega. } { apply IHk in H0. omega. } }
+Qed.
+
+Lemma search_correctness
       (g   : goal)
-      (k   : nat)      
+      (k   : nat)
       (HC  : closed_goal_in_context (first_nats k) g)
       (f   : gt_fun)
       (t   : trace)
       (HOP : op_sem (State (Leaf g empty_subst k)) t)
-      (HDA : in_denotational_analog t f) : exists f', forall n, In n (first_nats k) -> f n = f' n.
+      (HDA : in_denotational_analog t f) : in_denotational_sem_goal g f.
 Proof.
+  remember (State (Leaf g empty_subst k)) as st.
+  assert (in_denotational_sem_state st f).
+  { eapply search_correctness_generalized; eauto.
+    subst. constructor. constructor.
+    intros. apply HC in H. apply first_nats_less. auto. }
+  subst. inversion H. inversion Hst'. auto.
+Qed.
